
\documentclass[11pt]{article}
\usepackage{datetime}
\usepackage{color,array,graphics}
\usepackage{enumerate}
\usepackage[pdftex, colorlinks, linkcolor=red,citecolor=red,urlcolor=blue]{hyperref}
\usepackage{ulem}

\setlength{\parindent}{0cm}

\setlength{\parskip}{0.3cm plus4mm minus3mm}

\textwidth  6.5in
\oddsidemargin +0.0in
\evensidemargin +0.0in
\textheight 9.0in
\topmargin -0.5in

\usepackage{upquote,textcomp}
\usepackage{amssymb,amsmath,amsfonts,amsthm}
\usepackage{graphicx}
\usepackage{multicol}
\usepackage[T1]{fontenc}

\def\OR{\vee}
\def\AND{\wedge}
\def\imp{\rightarrow}

\DeclareSymbolFont{AMSb}{U}{msb}{m}{n}
\DeclareMathSymbol{\N}{\mathbin}{AMSb}{"4E}
\DeclareMathSymbol{\Z}{\mathbin}{AMSb}{"5A}
\DeclareMathSymbol{\R}{\mathbin}{AMSb}{"52}
\DeclareMathSymbol{\Q}{\mathbin}{AMSb}{"51}
\DeclareMathSymbol{\I}{\mathbin}{AMSb}{"49}
\DeclareMathSymbol{\C}{\mathbin}{AMSb}{"43}

\begin{document}
\thispagestyle{empty}   %% skips page number on the first page

\begin{center}
\large
\textbf{CSCI 2200 --- Foundations of Computer Science (FoCS) \\
Problem Set 3 (document version 1.0)}
\\Hayden Fuller
\end{center}


\begin{itemize}

\item \textbf{*Problem PS3.1.}
\\a)
\\we prove this with induction
\\$n=2$, $L_0=2$, $L_1=1$, $L_2=3$, $L_3=4$, $L_4=7$
\\$L_0+L_1+L_2=2+1+3=6=L_{2+2}-1=L_4-1=7-1=6$
\\so $L_0+L_1+L_2+...+L_n=L_{n+2}-1$ is true for $n=2$
\\assume $L_0+L_1+L_2+...+L_n=L_{n+2}-1$ is true
\\$L_0+L_1+L_2+...+L_n+L_{n+1}=L_{n+2+1}-1=L_{n+2+1-1}+L_{n+2+1-2}-1=L_{n+2}+L_{n+1}-1$
\\since  $L_0+L_1+L_2+...+L_n=L_{n+2}-1$, we can subtract from both sides which leaves us with $L_{n+1}=L_{n+1}$ which is true
\\therefore  $L_0+L_1+L_2+...+L_n=L_{n+2}-1$ is true
\\
\\b)
\\$F_0=0$, $F_1=1$, $F_2=1$, $F_3=2$, $F_4=3$
\\$n=2$, $L_2=F_{2-1}+F_{2+1}=F_1+F_3$, $3=1+2$
\\so $L_n=F_{n-1}+F_{n+1}$ is true for $n=2$
\\$n=3$, $L_3=F_{3-1}+F_{3+1}=F_2+F_4$, $4=1+3$
\\so $L_n=F_{n-1}+F_{n+1}$ is true for $n=3$
\\assume $L_n=F_{n-1}+F_{n+1}$ and  $L_{n+1}=F_{n+1-1}+F_{n+1+1}=F_{n}+F_{n+2}$ are true
\\$L_{n+2}=F_{n+2-1}+F_{n+2+1}=F_{n+1}+F_{n+3}$
\\$L_{n-1+2}+L_{n-2+2}=L_{n+1}+L_{n}=F_{n-1+1}+F_{n-2+1}+F_{n-1+3}+F_{n-2+3}=F_{n}+F_{n-1}+F_{n+2}+F_{n+1}$
\\$L_{n+1}+L_{n}=F_{n}+F_{n-1}+F_{n+2}+F_{n+1}$
\\$L_{n+1}=F_{n}+F_{n+2}$
\\therefore $L_n=F_{n-1}+F_{n+1}$ is true



\vspace{0.1in}

\item \textbf{*Problem PS3.2.}
\\we prove this with induction
\\$2+6+12+...+(n^2-n)=(n(n^2-1))/3$
\\$n=0$, $0^2-0=0=(0(0^2-1))/3=0$
\\ so $2+6+12+...+(n^2-n)=(n(n^2-1))/3$ is true for $n=0$
\\assume $2+6+12+...+(n^2-n)=(n(n^2-1))/3$ is true
\\$2+6+12+...+(n^2-n)+((n+1)^2-(n+1))=((n+1)((n+1)^2-1))/3$
\\$2+6+12+...+(n^2-n)+((n^2+2n+1-n-1))=((n+1)(n^2+2n+1-1))/3$
\\$(n(n^2-1))/3+(n^2+n)=((n+1)(n^2+2n))/3$
\\$(n^3-n)/3+(n^2+n)=(n^3+3n^2+2n)/3$
\\$(n^3-n)+(3n^2+3n)=(n^3+3n^2+2n)$
\\$n^3+3n^2+2n=n^3+3n^2+2n$ is true
\\therefore $2+6+12+...+(n^2-n)=(n(n^2-1))/3$ is true


\vspace{0.1in}

\item \textbf{*Problem 6.21.}
Prove that for $n\ge 1$, there is $k\ge 0$ and $l$ odd such that $n=2^kl$
\\we prove this by strong induction
\\if $n$ is odd, $l=n$ and $k=0$
\\if $n$ is even, it can be writen as $2j$, and $j<k$
\\if $n=2^kl \AND n=2j \imp j=2^{k_2}l$: $k_2=k+1$
\\
\\
\\

\end{itemize}

\end{document}























